restore the extraction for low-level spec

specs/experimental/rsapss/low-level/Spec.Bignum.Base.fst
@@ -4,6 +4,7 @@ open FStar.Mul
 open Spec.Lib.IntTypes
 open Spec.Lib.IntSeq
 open Spec.Lib.RawIntTypes
+open FStar.Math.Lemmas
 
 val eq_u8: a:uint8 -> b:uint8 -> Tot bool
 let eq_u8 a b = FStar.UInt8.(u8_to_UInt8 a =^ u8_to_UInt8 b)
@@ -32,27 +33,19 @@ let subborrow_u64 a b c =
       (if (lt_u64 a b) then u8 1 else u8 0) in
   (c, res)
 
+val lemma_mul_carry_add_64:
+  a:uint64 -> b:uint64 -> c:uint64 -> d:uint64 -> Lemma
+  (uint_v a * uint_v b + uint_v c + uint_v d < pow2 128)
+let lemma_mul_carry_add_64 a b c d =
+  let n = pow2 64 in
+  assert (uint_v a <= n - 1 /\ uint_v b <= n - 1 /\ uint_v c <= n - 1 /\ uint_v d <= n - 1);
+  assert (uint_v a * uint_v b + uint_v c + uint_v d <= (n - 1) * (n - 1) + (n - 1) + (n - 1));
+  assert ((n - 1) * (n - 1) + (n - 1) + (n - 1) == n * n - 1);
+  pow2_plus 64 64
+
 let mul_carry_add_u64 a b c d =
-  assume (uint_v #U64 a * uint_v #U64 b + uint_v #U64 c + uint_v #U64 d < pow2 128);
+  lemma_mul_carry_add_64 a b c d;
   let res = add #U128 (add #U128 (mul_wide a b) (to_u128 #U64 c)) (to_u128 #U64 d) in
   let r = to_u64 res in
   let c' = to_u64 (res >>. u32 64) in
   (c', r)
-
-(*
-val add_with_carry:
-  a:uint64 -> b:uint64 -> c:carry -> Pure (tuple2 carry uint64)
-  (requires (True))
-  (ensures (fun (c', r) -> uint_v r + uint_v c' * x_i 1 = uint_v a + uint_v b + uint_v c))
-  #reset-options "--z3rlimit 50 --max_fuel 0"
-let add_with_carry a b c =
-  let tmp = to_u128 a +! to_u128 b +! to_u128 c in
-  let r = to_u64 tmp in
-  assert (uint_v r = (uint_v a + uint_v b + uint_v c) % pow2 64);
-  let c' = to_u8 (tmp >>. (u32 64)) in
-  assert (uint_v c' = (uint_v a + uint_v b + uint_v c) / pow2 64);
-  lemma_div_mod (uint_v a + uint_v b + uint_v c) (pow2 64);
-  assert_norm (x_i 1 = pow2 64);
-  assert (uint_v c' == 0 \/ uint_v c' == 1);
-  (c', r)
-*)
